---
title: "Trig Cheat Sheet"
weight: 1
---

## Reciprocal Identities

{{< columns >}} <!-- begin -->
$$\sin(x)=\frac{1}{\csc(x)}$$
<---> <!-- separator -->
$$\cos(x)=\frac{1}{\sec(x)}$$
<---> <!-- separator -->
$$\tan(x)=\frac{\sin(x)}{\cos(x)}=\frac{1}{\cot(x)}$$
{{< /columns >}}

## Pythagorean Identities

{{< columns >}} <!-- begin -->
$$\sin^2(x) + \cos^2(x) = 1$$
<---> <!-- separator -->
$$1+\tan^2(x) = \sec^2(x)$$
<---> <!-- separator -->
$$1+\cot^2(x)=csc^2(x)$$
{{< /columns >}}

## Cofunction Identities

{{< columns >}} <!-- begin -->
$$\sin\Big(\frac{\pi}{2}-x\Big) = \cos(x)$$
$$\csc\Big(\frac{\pi}{2}-x\Big) = \sec(x)$$
<---> <!-- separator -->
$$\cos\Big(\frac{\pi}{2}-x\Big) = \sin(x)$$
$$\sec\Big(\frac{\pi}{2}-x\Big) = \csc(x)$$
<---> <!-- separator -->
$$\tan\Big(\frac{\pi}{2}-x\Big) = \cot(x)$$
$$\cot\Big(\frac{\pi}{2}-x\Big) = \tan(x)$$
{{< /columns >}}

## Even/Odd Identities

{{< columns >}} <!-- begin -->
$$ \sin(-x) = -\sin(x)$$
$$ \sec(-x) = \sec(x)$$
<---> <!-- separator -->
$$ \cos(-x) = \cos(x)$$
$$ \csc(-x) = -\csc(x)$$
<---> <!-- separator -->
$$ \tan(-x) = - \tan(x)$$
$$ \cot(-x) = -\cot(x)$$
{{< /columns >}}

## Sum and Difference Formulas

$$ \sin(u \pm v) = \sin(u) \cdot \cos(v) \pm \cos(u) \cdot \sin(v)$$
$$ \cos(u \pm v) = \cos(u) \cdot \cos(v) \pm \sin(u) \cdot \sin(v)$$

$$\tan(u \pm v) = \frac{\tan(u) \pm \tan(v)}{1 \mp \tan(u) \tan(v)}$$

## Double-Angle Formula

{{< columns >}} <!-- begin -->

$$ \sin(2u) = 2 \sin(u) \cos(u)$$
<---> <!-- separator -->
$$ \cos(2u) = 2 \cos^2(u) - 1$$
$$ ... = 1- 2 \sin^2(u) $$
$$ ... = \cos^2(u) - \sin^2(u) $$
<---> <!-- separator -->
$$ \tan(2u) = \frac{2 \tan(u)}{1 - \tan^2(u)}$$
{{< /columns >}}

## Power Reducing Formulas

{{< columns >}} <!-- begin -->
$$\sin^2(u) = \frac{1 - \cos(2u)}{2}$$
<---> <!-- separator -->
$$\cos^2(u) = \frac{1 + \cos(2u)}{2}$$
<---> <!-- separator -->
$$\tan^2(u) = \frac{1 - \cos(2u)}{1 + \cos(2u)}$$
{{< /columns >}}

## Sum to Product Formulas

$$\sin(u) + \sin(v) = 2\sin\bigg(\frac{u + v}{2}\bigg) \cos\bigg(\frac{u - v}{2}\bigg)\ \ \ \ \ \ \ \ \ \ \ \ \ \ \ $$
$$\sin(u) - \sin(v) = 2\cos\bigg(\frac{u + v}{2}\bigg) \sin\bigg(\frac{u - v}{2}\bigg)\ \ \ \ \ \ \ \ \ \ \ \ \ \ \ $$
$$\ \ \ \ \ \ \ \ \ \ \ \ \ \ \ \cos(u) + \cos(v) = 2\cos\bigg(\frac{u + v}{2}\bigg) \cos\bigg(\frac{u - v}{2}\bigg)$$
$$\ \ \ \ \ \ \ \ \ \ \ \ \ \ \ \cos(u) - \cos(v) = -2\sin\bigg(\frac{u + v}{2}\bigg) \sin\bigg(\frac{u - v}{2}\bigg)$$

## Product to Sum Formulas

$$\sin(u) \sin(v) = \frac{1}{2}\Big[\cos(u - v) - \cos(u + v)\Big]\ \ \ \ \ \ \ \ \ \ \ \ \ \ \ $$
$$\sin(u) \cos(v) = \frac{1}{2}\Big[\sin(u + v) + \sin(u - v)\Big]\ \ \ \ \ \ \ \ \ \ \ \ \ \ \ $$
$$\ \ \ \ \ \ \ \ \ \ \ \ \ \ \ \cos(u) \sin(v) = \frac{1}{2}\Big[\sin(u + v) - \sin(u - v)\Big]$$
$$\ \ \ \ \ \ \ \ \ \ \ \ \ \ \ \cos(u) \cos(v) = \frac{1}{2}\Big[\cos(u - v) + \cos(u + v)\Big]$$
